merkle: move node decoding to serde file

new/proof/github_com/sanjit_bhat/pav/merkle_proof/serde.v
@@ -1,7 +1,254 @@
 From New.proof.github_com.sanjit_bhat.pav Require Import prelude.
 From New.generatedproof.github_com.sanjit_bhat.pav Require Import merkle.
 
+From New.proof.github_com.sanjit_bhat.pav Require Import cryptoffi.
 From New.proof.github_com.sanjit_bhat.pav.merkle_proof Require Import base.
+
+Section proof.
+
+Inductive dec_node :=
+  | DecEmpty
+  | DecLeaf (label val : list w8)
+  | DecInner (hash0 hash1 : list w8)
+  | DecInvalid.
+
+Definition decode_leaf (data : list w8) : option (list w8 * list w8) :=
+  let rem0 := data in
+  match bool_decide (length rem0 >= 8%nat) with
+  | false => None
+  | _ =>
+    let label_len := uint.nat (le_to_u64 (take 8%nat rem0)) in
+    let rem1 := drop 8%nat rem0 in
+    match bool_decide (length rem1 >= label_len) with
+    | false => None
+    | _ =>
+      let label := take label_len rem1 in
+      let rem2 := drop label_len rem1 in
+      match bool_decide (length rem2 >= 8%nat) with
+      | false => None
+      | _ =>
+        let val_len := uint.nat (le_to_u64 (take 8%nat rem2)) in
+        let rem3 := drop 8%nat rem2 in
+        match bool_decide (length rem3 >= val_len) with
+        | false => None
+        | _ =>
+          let val := take val_len rem3 in
+          let rem4 := drop val_len rem3 in
+          match bool_decide (rem4 = []) with
+          | false => None
+          | _ => Some (label, val)
+          end
+        end
+      end
+    end
+  end.
+
+(* [decode_node] lets us compute one dec_node of a tree inversion. *)
+Definition decode_node (data : option $ list w8) :=
+  match data with
+  | None => DecInvalid
+  | Some d =>
+    match d with
+    | [] => DecInvalid
+    | tag :: d' =>
+      if decide (tag = emptyNodeTag ∧ d' = [])
+      then DecEmpty
+      else if decide (tag = leafNodeTag)
+      then
+        match decode_leaf d' with
+        | None => DecInvalid
+        | Some x => DecLeaf x.1 x.2
+        end
+      else if decide (tag = innerNodeTag ∧ Z.of_nat (length d') = 2 * cryptoffi.hash_len)
+      then
+        DecInner
+          (take (Z.to_nat cryptoffi.hash_len) d')
+          (drop (Z.to_nat cryptoffi.hash_len) d')
+      else DecInvalid
+    end
+  end.
+
+Lemma decode_empty_inj d :
+  decode_node d = DecEmpty →
+  d = Some [emptyNodeTag].
+Proof.
+  rewrite /decode_node. intros.
+  case_match; [|done].
+  case_match; [done|].
+  case_decide; [naive_solver|].
+  case_decide; [by case_match|].
+  by case_decide.
+Qed.
+
+Lemma decode_empty_det :
+  decode_node (Some [emptyNodeTag]) = DecEmpty.
+Proof.
+  simpl.
+  case_decide; [done|].
+  naive_solver.
+Qed.
+
+Lemma decode_leaf_inj_aux d l v :
+  decode_leaf d = Some (l, v) →
+  d = u64_le (W64 (length l)) ++ l ++ u64_le (W64 (length v)) ++ v.
+Proof.
+  rewrite /decode_leaf. intros.
+  case_bool_decide; [|done].
+  case_bool_decide; [|done].
+  case_bool_decide; [|done].
+  case_bool_decide; [|done].
+  case_bool_decide; [|done].
+  simplify_eq/=.
+  remember d as rem0.
+
+  rewrite -{1}(take_drop 8 rem0).
+  rewrite -{1}(take_drop 8 (_ ++ _ ++ _ ++ _)).
+  f_equal.
+  { rewrite take_app_length'; [|len].
+    rewrite length_take_le; [|lia].
+    rewrite w64_to_nat_id.
+    rewrite le_to_u64_le; [done|].
+    rewrite length_take. lia. }
+  remember (uint.nat (le_to_u64 (take 8 rem0))) as labelLen.
+  remember (drop 8 rem0) as rem1.
+
+  rewrite drop_app_length'; [|len].
+  rewrite -{1}(take_drop labelLen rem1).
+  f_equal.
+  remember (drop labelLen rem1) as rem2.
+
+  rewrite -{1}(take_drop 8 rem2).
+  rewrite -{1}(take_drop 8 (_ ++ _)).
+  f_equal.
+  { rewrite take_app_length'; [|len].
+    rewrite length_take_le; [|lia].
+    rewrite w64_to_nat_id.
+    rewrite le_to_u64_le; [done|].
+    rewrite length_take. lia. }
+  remember (uint.nat (le_to_u64 (take 8 rem2))) as valLen.
+  remember (drop 8 rem2) as rem3.
+
+  rewrite drop_app_length'; [|len].
+  rewrite -{1}(take_drop valLen rem3).
+  rewrite H4.
+  by list_simplifier.
+Qed.
+
+Lemma decode_leaf_inj d l v :
+  decode_node d = DecLeaf l v →
+  d =
+  Some $
+    leafNodeTag ::
+    u64_le (W64 (length l)) ++ l ++
+    u64_le (W64 (length v)) ++ v.
+Proof.
+  rewrite /decode_node. intros.
+  case_match; [|done].
+  case_match; [done|].
+  case_decide; [naive_solver|].
+  case_decide. 2: { by case_decide. }
+  case_match; [|done].
+  destruct p. simplify_eq/=.
+  opose proof (decode_leaf_inj_aux _ _ _ _) as Heq; [done|].
+  by rewrite Heq.
+Qed.
+
+Lemma decode_leaf_det_aux l v :
+  length l < 2^64 →
+  length v < 2^64 →
+  decode_leaf (
+    u64_le (W64 (length l)) ++ l ++
+    u64_le (W64 (length v)) ++ v
+  ) = Some (l, v).
+Proof.
+  intros. rewrite /decode_leaf.
+  repeat (rewrite take_app_length'; [|len]).
+  rewrite u64_le_to_word.
+  repeat (rewrite drop_app_length'; [|len]).
+  repeat (rewrite take_app_length'; [|len]).
+  rewrite u64_le_to_word.
+  rewrite take_ge; [|word].
+  rewrite drop_ge; [|word].
+
+  case_bool_decide as Hif.
+  2: { revert Hif. len. }
+  clear Hif.
+  case_bool_decide as Hif.
+  2: { revert Hif. len. }
+  clear Hif.
+  case_bool_decide as Hif.
+  2: { revert Hif. len. }
+  clear Hif.
+  case_bool_decide as Hif.
+  2: { revert Hif. len. }
+  clear Hif.
+  by case_bool_decide.
+Qed.
+
+Lemma decode_leaf_det l v :
+  length l < 2^64 →
+  length v < 2^64 →
+  decode_node (
+    Some $ leafNodeTag ::
+    u64_le (W64 (length l)) ++ l ++
+    u64_le (W64 (length v)) ++ v
+  ) = DecLeaf l v.
+Proof.
+  intros. simpl.
+  case_decide; [naive_solver|].
+  case_decide; [|done].
+  by rewrite decode_leaf_det_aux.
+Qed.
+
+Lemma decode_inner_inj d h0 h1 :
+  decode_node d = DecInner h0 h1 →
+  d = Some $ innerNodeTag :: h0 ++ h1 ∧
+    Z.of_nat $ length h0 = cryptoffi.hash_len ∧
+    Z.of_nat $ length h1 = cryptoffi.hash_len.
+Proof.
+  rewrite /decode_node. intros.
+  case_match; [|done].
+  case_match; [done|].
+  case_decide; [naive_solver|].
+  case_decide. { by case_match. }
+  case_decide; [|done].
+  destruct_and!.
+  simplify_eq/=.
+  split; [|len].
+  by rewrite take_drop.
+Qed.
+
+Lemma decode_inner_det h0 h1 :
+  Z.of_nat $ length h0 = cryptoffi.hash_len →
+  Z.of_nat $ length h1 = cryptoffi.hash_len →
+  decode_node (Some $ innerNodeTag :: h0 ++ h1) = DecInner h0 h1.
+Proof.
+  intros. simpl.
+  case_decide; [len|].
+  case_decide; [done|].
+  case_decide.
+  2: { intuition. revert H3. len. }
+  rewrite take_app_length'; [|lia].
+  by rewrite drop_app_length'; [|lia].
+Qed.
+
+(* for every node, there's only one data that decodes to it. *)
+Lemma decode_node_inj n d0 d1 :
+  n = decode_node d0 →
+  n = decode_node d1 →
+  n ≠ DecInvalid →
+  d0 = d1 ∧ is_Some d1.
+Proof.
+  intros. destruct n; try done.
+  - opose proof (decode_empty_inj d0 _) as ->; [done|].
+    by opose proof (decode_empty_inj d1 _) as ->.
+  - opose proof (decode_leaf_inj d0 _ _ _) as ->; [done|].
+    by opose proof (decode_leaf_inj d1 _ _ _) as ->.
+  - opose proof (decode_inner_inj d0 _ _ _) as [-> ?]; [done|].
+    by opose proof (decode_inner_inj d1 _ _ _) as [-> ?].
+Qed.
+
+End proof.
 
 Module MerkleProof.
 Record t :=
